src/Expr.v
@@ -595,20 +595,13 @@ Module Renaming.
   Definition renamings_inv (r r' : renaming) := forall (x : id), rename_id r (rename_id r' x) = x.
 
   Lemma renaming_inv (r : renaming) : exists (r' : renaming), renamings_inv r' r.
-  Proof.
-    destruct r. unfold Bijective in b. inversion b. inversion_clear H.
-    assert (B: Bijective x0). unfold Bijective. exists x. split; assumption.
-    exists (exist _ x0 B).
-    unfold renamings_inv. intro x1. simpl. auto.
-  Qed.
+  Proof. destruct r, b, a. exists (exist _ _ (ex_intro _ x (conj e0 e))). auto. Qed.
 
   Lemma renaming_inv2 (r : renaming) : exists (r' : renaming), renamings_inv r r'.
-  Proof.
-    destruct r. unfold Bijective in b. inversion b. inversion_clear H.
-    assert (B: Bijective x0). unfold Bijective. exists x. split; assumption.
-    exists (exist _ x0 B).
-    unfold renamings_inv. intro x1. simpl. auto.
-  Qed.
+  Proof. destruct r, b, a. exists (exist _ _ (ex_intro _ x (conj e0 e))). auto. Qed.
+
+  Lemma renamings_symm r r' (Hinv : renamings_inv r r') : renamings_inv r' r.
+  Proof. destruct r, b, a, r', b, a. unfold renamings_inv in *. simpl in *. congruence. Qed.
 
   Fixpoint rename_expr (r : renaming) (e : expr) : expr :=
     match e with
@@ -621,7 +614,12 @@ Module Renaming.
     (r r' : renaming)
     (Hinv : renamings_inv r r')
     (e    : expr) : rename_expr r (rename_expr r' e) = e.
-  Proof. admit. Admitted.
+  Proof.
+    dependent induction e; simpl.
+    * reflexivity.
+    * rewrite Hinv. reflexivity.
+    * rewrite IHe1, IHe2. reflexivity.
+  Qed.
 
   Fixpoint rename_state (r : renaming) (st : state Z) : state Z :=
     match st with
@@ -634,7 +632,12 @@ Module Renaming.
     (r r' : renaming)
     (Hinv : renamings_inv r r')
     (st   : state Z) : rename_state r (rename_state r' st) = st.
-  Proof. admit. Admitted.
+  Proof.
+    dependent induction st; simpl.
+    * reflexivity.
+    * destruct a, r, b, a, r', b, a. unfold renamings_inv in *. simpl in *.
+      rewrite IHst; auto. congruence.
+  Qed.
 
   Lemma bijective_injective (f : id -> id) (BH : Bijective f) : Injective f.
   Proof. inversion BH. inversion H. congruence. Qed.
